BananasLanguage.thy
@@ -1,0 +1,52 @@
+theory BananasLanguage
+imports Main
+begin
+
+type_synonym name = string
+
+datatype type = 
+  Void ("\<zero>")
+| Unit ("\<one>")
+| Poly nat
+| Prod type type (infixr "\<otimes>" 85)
+| Sum type type (infixr "\<oplus>" 80)
+| Func type type (infixr "\<hookrightarrow>" 70)
+| Fix funct ("\<mu>")
+and funct =
+  Id
+| K type
+| ProdF funct funct (infixr "\<Otimes>" 85)
+| SumF funct funct (infixr "\<Oplus>" 80)
+
+datatype expr = 
+  Identity ("\<epsilon>") | Const val ("\<kappa>") | Comp expr expr (infixr "\<cdot>" 65)
+| Proj1 ("\<pi>\<^sub>1") | Proj2 ("\<pi>\<^sub>2") | Duplicate ("\<Theta>") | Pairwise expr expr (infixr "\<parallel>" 85)
+| Injl ("\<iota>\<^sub>l") | Injr ("\<iota>\<^sub>r") | Strip ("\<Xi>") |  Case expr expr (infixr "\<bar>" 80)
+| Distribute ("\<rhd>")
+| Apply ("$") | Arrow expr expr (infixl "\<leftarrow>" 70)
+| Inj name ("\<succ>\<^bsub>_\<^esub>") | Outj name ("\<prec>\<^bsub>_\<^esub>")
+| Cata expr name ("\<lparr> _ \<rparr>\<^bsub>_\<^esub>") | Ana expr name ("\<lbrakk> _ \<rbrakk>\<^bsub>_\<^esub>")
+| Var name
+and val = 
+  UnitV
+| PairV val val 
+| InlV val | InrV val
+| FunV expr
+| InjV name val 
+
+datatype decl = 
+  TypeDecl name "(name \<times> name list) list"
+| ValDecl name val
+| ExprDecl name expr
+
+primrec binders\<^sub>d :: "decl \<Rightarrow> name set" where
+  "binders\<^sub>d (TypeDecl x cts) = insert x (fst ` set cts)"
+| "binders\<^sub>d (ValDecl x v) = {x}"
+| "binders\<^sub>d (ExprDecl x e) = {x}"
+
+fun binders :: "decl list \<Rightarrow> name set" where
+  "binders \<Lambda> = \<Union> (binders\<^sub>d ` set \<Lambda>)"
+
+datatype prog = Prog "decl list" expr val
+
+end
