BananasStatics.thy
@@ -1,0 +1,146 @@
+theory BananasStatics
+imports BananasLanguage
+begin
+
+record static_environment = 
+  var\<^sub>e_type :: "name \<rightharpoonup> type \<times> type" 
+  var\<^sub>v_type :: "name \<rightharpoonup> type list \<times> type" 
+  var\<^sub>t_type :: "name \<rightharpoonup> funct"
+
+definition empty_static :: static_environment where
+  "empty_static = \<lparr> var\<^sub>e_type = Map.empty, var\<^sub>v_type = Map.empty, var\<^sub>t_type = Map.empty \<rparr>"
+
+definition extend\<^sub>e\<^sub>s :: "name \<Rightarrow> type \<times> type \<Rightarrow> static_environment \<Rightarrow> static_environment" where
+  "extend\<^sub>e\<^sub>s x t \<Gamma> = \<Gamma>\<lparr> var\<^sub>e_type := var\<^sub>e_type \<Gamma>(x \<mapsto> t) \<rparr>"
+
+definition extend\<^sub>v\<^sub>s :: "name \<Rightarrow> type list \<times> type \<Rightarrow> static_environment \<Rightarrow> static_environment" where
+  "extend\<^sub>v\<^sub>s x t \<Gamma> = \<Gamma>\<lparr> var\<^sub>v_type := var\<^sub>v_type \<Gamma>(x \<mapsto> t) \<rparr>"
+
+definition combine\<^sub>s :: "static_environment \<Rightarrow> static_environment \<Rightarrow> static_environment" where
+  "combine\<^sub>s \<Gamma> \<Gamma>' = \<lparr> 
+      var\<^sub>e_type = var\<^sub>e_type \<Gamma> ++ var\<^sub>e_type \<Gamma>', 
+      var\<^sub>v_type = var\<^sub>v_type \<Gamma> ++ var\<^sub>v_type \<Gamma>', 
+      var\<^sub>t_type = var\<^sub>t_type \<Gamma> ++ var\<^sub>t_type \<Gamma>' \<rparr>"
+
+definition domain\<^sub>s :: "static_environment \<Rightarrow> name set" where
+  "domain\<^sub>s \<Gamma> = dom (var\<^sub>e_type \<Gamma>) \<union> dom (var\<^sub>v_type \<Gamma>) \<union> dom (var\<^sub>t_type \<Gamma>)"
+
+fun apply_functor_type :: "type \<Rightarrow> funct \<Rightarrow> type" (infixl "\<star>" 75) where
+  "t \<star> Id = t"
+| "t \<star> K t' = t'"
+| "t \<star> f\<^sub>1 \<Otimes> f\<^sub>2 = (t \<star> f\<^sub>1) \<otimes> (t \<star> f\<^sub>2)"
+| "t \<star> f\<^sub>1 \<Oplus> f\<^sub>2 = (t \<star> f\<^sub>1) \<oplus> (t \<star> f\<^sub>2)"
+
+inductive typecheck\<^sub>e :: "static_environment \<Rightarrow> expr \<Rightarrow> type \<Rightarrow> type \<Rightarrow> bool" (infix "\<turnstile> _ : _ \<rightarrow>" 60)
+      and typecheck\<^sub>v :: "static_environment \<Rightarrow> val \<Rightarrow> type \<Rightarrow> bool" (infix "\<turnstile> _ :" 60) where
+  tc_id [simp]: "\<Gamma> \<turnstile> \<epsilon> : t \<rightarrow> t"
+| tc_con [simp]: "\<Gamma> \<turnstile> v : t\<^sub>2 \<Longrightarrow> \<Gamma> \<turnstile> \<kappa> v : t\<^sub>1 \<rightarrow> t\<^sub>2"
+| tc_comp [simp]: "\<Gamma> \<turnstile> f : t\<^sub>2 \<rightarrow> t\<^sub>3 \<Longrightarrow> \<Gamma> \<turnstile> g : t\<^sub>1 \<rightarrow> t\<^sub>2 \<Longrightarrow> \<Gamma> \<turnstile> f \<cdot> g : t\<^sub>1 \<rightarrow> t\<^sub>3"
+| tc_fst [simp]: "\<Gamma> \<turnstile> \<pi>\<^sub>1 : t\<^sub>1 \<otimes> t\<^sub>2 \<rightarrow> t\<^sub>1"
+| tc_snd [simp]: "\<Gamma> \<turnstile> \<pi>\<^sub>2 : t\<^sub>1 \<otimes> t\<^sub>2 \<rightarrow> t\<^sub>2"
+| tc_tup [simp]: "\<Gamma> \<turnstile> \<Theta> : t \<rightarrow> t \<otimes> t"
+| tc_pair [simp]: "\<Gamma> \<turnstile> f\<^sub>1 : t\<^sub>1 \<rightarrow> t\<^sub>2 \<Longrightarrow> \<Gamma> \<turnstile> f\<^sub>2 : t\<^sub>3 \<rightarrow> t\<^sub>4 \<Longrightarrow> 
+    \<Gamma> \<turnstile> f\<^sub>1 \<parallel> f\<^sub>2 : t\<^sub>1 \<otimes> t\<^sub>3 \<rightarrow> t\<^sub>2 \<otimes> t\<^sub>4"
+| tc_inl [simp]: "\<Gamma> \<turnstile> \<iota>\<^sub>l : t\<^sub>1 \<rightarrow> t\<^sub>1 \<oplus> t\<^sub>2"
+| tc_inr [simp]: "\<Gamma> \<turnstile> \<iota>\<^sub>r : t\<^sub>2 \<rightarrow> t\<^sub>1 \<oplus> t\<^sub>2"
+| tc_str [simp]: "\<Gamma> \<turnstile> \<Xi> : t\<^sub>1 \<oplus> t\<^sub>1 \<rightarrow> t\<^sub>1"
+| tc_case [simp]: "\<Gamma> \<turnstile> f\<^sub>l : t\<^sub>1 \<rightarrow> t\<^sub>3 \<Longrightarrow> \<Gamma> \<turnstile> f\<^sub>r : t\<^sub>2 \<rightarrow> t\<^sub>4 \<Longrightarrow> 
+    \<Gamma> \<turnstile> f\<^sub>l \<bar> f\<^sub>r : t\<^sub>1 \<oplus> t\<^sub>2 \<rightarrow> t\<^sub>3 \<oplus> t\<^sub>4"
+| tc_dst [simp]: "\<Gamma> \<turnstile> \<rhd> : (t\<^sub>1 \<oplus> t\<^sub>2) \<otimes> t\<^sub>3 \<rightarrow> t\<^sub>1 \<otimes> t\<^sub>3 \<oplus> t\<^sub>2 \<otimes> t\<^sub>3"
+| tc_app [simp]: "\<Gamma> \<turnstile> $ : (t\<^sub>1 \<hookrightarrow> t\<^sub>2) \<otimes> t\<^sub>1 \<rightarrow> t\<^sub>2"
+| tc_arr [simp]: "\<Gamma> \<turnstile> f : t\<^sub>1 \<rightarrow> t\<^sub>2 \<Longrightarrow> \<Gamma> \<turnstile> g : t\<^sub>3 \<rightarrow> t\<^sub>4 \<Longrightarrow> 
+    \<Gamma> \<turnstile> g \<leftarrow> f : t\<^sub>2 \<hookrightarrow> t\<^sub>3 \<rightarrow> t\<^sub>1 \<hookrightarrow> t\<^sub>4"
+| tc_inj [simp]: "var\<^sub>t_type \<Gamma> n = Some F \<Longrightarrow> \<Gamma> \<turnstile> \<succ>\<^bsub>n\<^esub> : \<mu> F \<star> F \<rightarrow> \<mu> F"
+| tc_outj [simp]: "var\<^sub>t_type \<Gamma> n = Some F \<Longrightarrow> \<Gamma> \<turnstile> \<prec>\<^bsub>n\<^esub> : \<mu> F \<rightarrow> \<mu> F \<star> F"
+| tc_cata [simp]: "var\<^sub>t_type \<Gamma> n = Some F \<Longrightarrow> \<Gamma> \<turnstile> f : t \<star> F \<rightarrow> t \<Longrightarrow> \<Gamma> \<turnstile> \<lparr> f \<rparr>\<^bsub>n\<^esub> : \<mu> F \<rightarrow> t"
+| tc_ana [simp]: "var\<^sub>t_type \<Gamma> n = Some F \<Longrightarrow> \<Gamma> \<turnstile> f : t \<rightarrow> t \<star> F \<Longrightarrow> \<Gamma> \<turnstile> \<lbrakk> f \<rbrakk>\<^bsub>n\<^esub> : t \<rightarrow> \<mu> F"
+| tc_var [simp]: "var\<^sub>e_type \<Gamma> x = Some (t\<^sub>1, t\<^sub>2) \<Longrightarrow> \<Gamma> \<turnstile> Var x : t\<^sub>1 \<rightarrow> t\<^sub>2"
+
+| tcv_unit [simp]: "\<Gamma> \<turnstile> UnitV : \<one>"
+| tcv_pair [simp]: "\<Gamma> \<turnstile> v\<^sub>1 : t\<^sub>1 \<Longrightarrow> \<Gamma> \<turnstile> v\<^sub>2 : t\<^sub>2 \<Longrightarrow> \<Gamma> \<turnstile> PairV v\<^sub>1 v\<^sub>2 : t\<^sub>1 \<otimes> t\<^sub>2"
+| tcv_inl [simp]: "\<Gamma> \<turnstile> v : t\<^sub>1 \<Longrightarrow> \<Gamma> \<turnstile> InlV v : t\<^sub>1 \<oplus> t\<^sub>2"
+| tcv_inr [simp]: "\<Gamma> \<turnstile> v : t\<^sub>2 \<Longrightarrow> \<Gamma> \<turnstile> InrV v : t\<^sub>1 \<oplus> t\<^sub>2"
+| tcv_fun [simp]: "\<Gamma> \<turnstile> e : t\<^sub>1 \<rightarrow> t\<^sub>2 \<Longrightarrow> \<Gamma> \<turnstile> FunV e : t\<^sub>1 \<hookrightarrow> t\<^sub>2"
+| tcv_inj [simp]: "var\<^sub>t_type \<Gamma> n = Some F \<Longrightarrow> \<Gamma> \<turnstile> v : \<mu> F \<star> F \<Longrightarrow> \<Gamma> \<turnstile> InjV n v : \<mu> F"
+
+inductive_cases [elim]: "\<Gamma> \<turnstile> \<epsilon> : t \<rightarrow> t'"
+inductive_cases [elim]: "\<Gamma> \<turnstile> \<kappa> v : t \<rightarrow> t'"
+inductive_cases [elim]: "\<Gamma> \<turnstile> f \<cdot> g : t \<rightarrow> t'"
+inductive_cases [elim]: "\<Gamma> \<turnstile> \<pi>\<^sub>1 : t \<rightarrow> t'"
+inductive_cases [elim]: "\<Gamma> \<turnstile> \<pi>\<^sub>2 : t \<rightarrow> t'"
+inductive_cases [elim]: "\<Gamma> \<turnstile> \<Theta> : t \<rightarrow> t'"
+inductive_cases [elim]: "\<Gamma> \<turnstile> f\<^sub>l \<parallel> f\<^sub>r : t \<rightarrow> t'"
+inductive_cases [elim]: "\<Gamma> \<turnstile> \<iota>\<^sub>l : t \<rightarrow> t'"
+inductive_cases [elim]: "\<Gamma> \<turnstile> \<iota>\<^sub>r : t \<rightarrow> t'"
+inductive_cases [elim]: "\<Gamma> \<turnstile> \<Xi> : t \<rightarrow> t'"
+inductive_cases [elim]: "\<Gamma> \<turnstile> f\<^sub>l \<bar> f\<^sub>r : t \<rightarrow> t'"
+inductive_cases [elim]: "\<Gamma> \<turnstile> \<rhd> : t \<rightarrow> t'"
+inductive_cases [elim]: "\<Gamma> \<turnstile> $ : t \<rightarrow> t'"
+inductive_cases [elim]: "\<Gamma> \<turnstile> g \<leftarrow> f : t \<rightarrow> t'"
+inductive_cases [elim]: "\<Gamma> \<turnstile> \<prec>\<^bsub>n\<^esub> : t \<rightarrow> t'"
+inductive_cases [elim]: "\<Gamma> \<turnstile> \<succ>\<^bsub>n\<^esub> : t \<rightarrow> t'"
+inductive_cases [elim]: "\<Gamma> \<turnstile> \<lparr> f \<rparr>\<^bsub>n\<^esub> : t \<rightarrow> t'"
+inductive_cases [elim]: "\<Gamma> \<turnstile> \<lbrakk> f \<rbrakk>\<^bsub>n\<^esub> : t \<rightarrow> t'"
+inductive_cases [elim]: "\<Gamma> \<turnstile> Var x : t \<rightarrow> t'"
+
+inductive_cases [elim]: "\<Gamma> \<turnstile> UnitV : t"
+inductive_cases [elim]: "\<Gamma> \<turnstile> PairV v\<^sub>1 v\<^sub>2 : t"
+inductive_cases [elim]: "\<Gamma> \<turnstile> InrV v : t"
+inductive_cases [elim]: "\<Gamma> \<turnstile> InlV v : t"
+inductive_cases [elim]: "\<Gamma> \<turnstile> FunV e : t"
+inductive_cases [elim]: "\<Gamma> \<turnstile> InjV f v : t"
+
+inductive typecheck\<^sub>c\<^sub>e :: "static_environment \<Rightarrow> funct \<Rightarrow> (name \<times> name list) list \<Rightarrow> 
+    (name \<rightharpoonup> type \<times> type) \<Rightarrow> bool" where
+  "typecheck\<^sub>c\<^sub>e \<Gamma> F [] Map.empty" 
+| "typecheck\<^sub>c\<^sub>e \<Gamma> F cts \<Gamma>' \<Longrightarrow> those (map (map_option \<mu> o var\<^sub>t_type \<Gamma>) ts) = Some ts' \<Longrightarrow> 
+    typecheck\<^sub>c\<^sub>e \<Gamma> F ((x, ts) # cts) (\<Gamma>'(x \<mapsto> (foldr (op \<otimes>) ts' \<one>, \<mu> F)))"
+
+definition typecheck\<^sub>c\<^sub>v :: "funct \<Rightarrow> (name \<times> name list) list \<Rightarrow> (name \<rightharpoonup> type list \<times> type)" where
+  "typecheck\<^sub>c\<^sub>v F cts x = (if x \<in> fst ` set cts then Some (\<mu> F) else None)"
+
+fun typecheck\<^sub>c\<^sub>t_arg :: "static_environment \<Rightarrow> name \<Rightarrow> name \<Rightarrow> funct option" where
+  "typecheck\<^sub>c\<^sub>t_arg \<Gamma> tn t = (if t = tn then Some Id else map_option (K o \<mu>) (var\<^sub>t_type \<Gamma> t))"
+
+primrec typecheck\<^sub>c\<^sub>t :: "static_environment \<Rightarrow> name \<Rightarrow> name \<times> name list \<Rightarrow> funct option" where
+  "typecheck\<^sub>c\<^sub>t \<Gamma> tn (x, ts) = 
+    map_option (\<lambda>fs. foldr (op \<Otimes>) fs (K \<one>)) (those (map (typecheck\<^sub>c\<^sub>t_arg \<Gamma> tn) ts))"
+
+definition typecheck\<^sub>c\<^sub>t\<^sub>s :: "static_environment \<Rightarrow> name \<Rightarrow> (name \<times> name list) list \<Rightarrow> funct option" 
+    where
+  "typecheck\<^sub>c\<^sub>t\<^sub>s \<Gamma> x cts = 
+    map_option (\<lambda>fs. foldr (op \<Oplus>) fs (K \<zero>)) (those (map (typecheck\<^sub>c\<^sub>t \<Gamma> x) cts))"
+
+inductive typecheck\<^sub>d\<^sub>t :: "static_environment \<Rightarrow> name \<Rightarrow> (name \<times> name list) list \<Rightarrow> 
+    static_environment \<Rightarrow> bool" where
+  "typecheck\<^sub>c\<^sub>t\<^sub>s \<Gamma> n cts = Some F \<Longrightarrow> typecheck\<^sub>c\<^sub>e \<Gamma> F cts \<Gamma>' \<Longrightarrow> 
+      typecheck\<^sub>d\<^sub>t \<Gamma> n cts \<lparr> var\<^sub>e_type = \<Gamma>', 
+                            var\<^sub>v_type = typecheck\<^sub>c\<^sub>v F cts, 
+                            var\<^sub>t_type = [n \<mapsto> F] \<rparr>"
+
+inductive typecheck_decl :: "static_environment \<Rightarrow> decl \<Rightarrow> static_environment \<Rightarrow> bool" 
+    (infix "\<Turnstile> _ :" 60) where
+  tcd_type [simp]: "typecheck\<^sub>d\<^sub>t \<Gamma> x cts \<Gamma>' \<Longrightarrow> \<Gamma> \<Turnstile> TypeDecl x cts : combine\<^sub>s \<Gamma> \<Gamma>'"
+| tcd_val [simp]: "\<Gamma> \<turnstile> v : t \<Longrightarrow> \<Gamma> \<Turnstile> ValDecl x v : extend\<^sub>v\<^sub>s x ([], t) \<Gamma>"
+| tcd_expr [simp]: "\<Gamma> \<turnstile> e : t\<^sub>1 \<rightarrow> t\<^sub>2 \<Longrightarrow> \<Gamma> \<Turnstile> ExprDecl x e : extend\<^sub>e\<^sub>s x (t\<^sub>1, t\<^sub>2) \<Gamma>"
+
+inductive_cases [elim]: "\<Gamma> \<Turnstile> TypeDecl x F : \<Gamma>'"
+inductive_cases [elim]: "\<Gamma> \<Turnstile> ValDecl x v : \<Gamma>'"
+inductive_cases [elim]: "\<Gamma> \<Turnstile> ExprDecl x e : \<Gamma>'"
+
+inductive typecheck_decls :: "static_environment \<Rightarrow> decl list \<Rightarrow> static_environment \<Rightarrow> bool" 
+    (infix "\<Turnstile> _ ::" 60) where
+  tcd_nil [simp]: "\<Gamma> \<Turnstile> [] :: \<Gamma>"
+| tcd_cons [simp]: "\<Gamma> \<Turnstile> \<delta> : \<Gamma>' \<Longrightarrow> binders\<^sub>d \<delta> \<inter> domain\<^sub>s \<Gamma> = {} \<Longrightarrow> \<Gamma>' \<Turnstile> \<Lambda> :: \<Gamma>'' \<Longrightarrow> 
+    \<Gamma> \<Turnstile> \<delta> # \<Lambda> :: \<Gamma>''"
+
+inductive_cases [elim]: "\<Gamma> \<Turnstile> [] :: \<Gamma>'"
+inductive_cases [elim]: "\<Gamma> \<Turnstile> \<delta> # \<Lambda> :: \<Gamma>'"
+
+inductive typecheck_prog :: "prog \<Rightarrow> static_environment \<Rightarrow> type \<Rightarrow> bool" (infix "\<TTurnstile> _ \<rightarrow> " 60) where
+  tcp_prog [simp]: "empty_static \<Turnstile> \<Lambda> :: \<Gamma> \<Longrightarrow> \<Gamma> \<turnstile> e : t\<^sub>1 \<rightarrow> t\<^sub>2 \<Longrightarrow> \<Gamma> \<turnstile> v : t\<^sub>1 \<Longrightarrow> 
+    Prog \<Lambda> e v \<TTurnstile> \<Gamma> \<rightarrow> t\<^sub>2"
+
+inductive_cases [elim]: "Prog \<Lambda> e v \<TTurnstile> \<Gamma>  \<rightarrow> t"
+
+end
